Orderedtree/Basic.lean
@@ -1,3 +1,6 @@
 import Orderedtree.DOrderedTree.Internal.Impl
+import Orderedtree.DOrderedTree.Internal.Model
+import Orderedtree.DOrderedTree.Internal.WF
 import Orderedtree.DOrderedTree.Raw
+import Orderedtree.DOrderedTree.Basic
 import Orderedtree.Examples.InversionCount
